\documentclass[]{report}


% Title Page
\title{Two step nitrification model study}
\author{Pablo Ugalde Salas}
\usepackage{amssymb}%% The amsthm package provides extended theorem environments
\usepackage{amsthm}
\usepackage{amsmath}
\usepackage{algorithm2e}
\usepackage{graphicx}
\usepackage{subcaption}
\usepackage{hyperref}
\usepackage{xcolor}
\usepackage[version=4]{mhchem}
\newcommand{\N}{\mathbb{N}}
\newcommand{\R}{\mathbb{R}}
\newcommand{\I}{\mathcal{I}}
\newcommand{\diag}{\textbf{diag}}
\newtheorem{defn}{Definition}
\newtheorem{hypo}{H}
\newtheorem{lemma}{Lemma}
\newtheorem{theo}{Theorem}

\begin{document}
\maketitle


\begin{align}
\label{Reaction1} \tag{R G1} 	s_1 \stackrel{\mu_1(s,x)}{\longrightarrow} s_2 + y_1x_1  \\
\label{Reaction2} \tag{R G2} s_2\stackrel{\mu_2(s,x)}{\longrightarrow} s_3 + y_2x_2 
\end{align}

\begin{align} 
\dot{x_1} =& \left(\mu_1(s,x) -D \right)x_1  \label{x_1} \\
\dot{x_2} =& \left(\mu_2(s,x) -D \right)x_2  \label{x_2}\\
\dot{s_1} =& \displaystyle (s_{in}-s_1)D- k_1\mu_1(s,x) x_1  \\
\dot{s_2} = & \displaystyle -s_2D+ k_1\mu_1(s,x)x_1 -k_2\mu_2(s,x) x_2  \\
\dot{s_3} =&  \displaystyle -s_3D+ k_2\mu_2(s,x) x_2 
\end{align}	

\textbf{Case 1:}
\begin{align}
\mu_1(s,x) =  \bar{\mu}_1 \dfrac{s_1}{K_1 + s_1} \\
\mu_2(s,x) =  \bar{\mu}_2 \dfrac{s_2}{K_1 + s_2} 
\end{align}

\textbf{Equilibrium points}
It is assumed that the points here presented are non-negative.  Three cases can take place:

\textbf{Coexistence:}
From \eqref{x_1} one gets:
\begin{align}
s_1^{eq} &= \frac{K_1D}{\bar{\mu}_1 - D} \\
x_1^{eq} &= \frac{s_{in} - s_1^{eq}}{k_1} \\
s_2^{eq} &= \frac{K_2D}{\bar{\mu}_2 - D} \\
x_2^{eq} &=\frac{s_{in} - s_1^{eq}-s_2^{eq}}{k_2}\\
s_3^{eq} &= s_{in} - s_1^{eq}-s_2^{eq} 
\end{align}

\textbf{Washout of $x_2$}
\begin{align}
s_1^{eq} &= \frac{K_1D}{\bar{\mu}_1 - D} \\
x_1^{eq} &= \frac{s_{in} - \frac{K_1D}{\bar{\mu}_1 - D}}{k_1} \\
s_2^{eq} &= s_{in} - s_1^{eq} \\
x_2^{eq} &=0 \\
s_3^{eq} &= 0 
\end{align}

\textbf{Washout}
\begin{align}
s_1^{eq} &= s_{in} \\
x_1^{eq} &= 0 \\
s_2^{eq} &= 0 \\
x_2^{eq} &=0 \\
s_3^{eq} &= 0 
\end{align}

\textbf{Jacobian of the system:}
\begin{align}
J_{11} & = \bar{\mu}_1 \dfrac{s_1}{K_1 + s_1} -D \\
J_{12} & = 0 \\
J_{13} & = \bar{\mu}_1 \dfrac{K_1}{(K_1 + s_1)^2}x_1 \\
J_{14} & = 0 \\
J_{15} & = 0 \\
J_{21} & = 0 \\
J_{22} & = \bar{\mu}_1 \dfrac{s_2}{K_2 + s_2} -D \\
J_{23} & = 0 \\
J_{24} & = \bar{\mu}_2 \dfrac{K_1}{(K_1 + s_2)^2}x_2  \\
J_{25} & = 0 \\
J_{31} & = -k_1\bar{\mu}_1 \dfrac{s_1}{K_1 + s_1} \\
J_{32} & = 0 \\
J_{33} & = -D -k_1\bar{\mu}_1 \dfrac{K_1}{(K_1 + s_1)^2}x_1 \\
J_{34} & = 0 \\
J_{35} & = 0 \\
J_{41} & = k_1\bar{\mu}_1 \dfrac{s_1}{K_1 + s_1} \\
J_{42} & = -k_2\bar{\mu}_2 \dfrac{s_2}{K_2 + s_2} \\
J_{43} & = k_1  \bar{\mu}_1 \dfrac{K_1}{(K_1 + s_1)^2}x_1 \\
J_{44} & = -D-k_2 \bar{\mu}_2 \dfrac{K_2}{(K_2 + s_2)^2}x_2 \\
J_{45} & = 0 \\
J_{51} & = 0 \\
J_{52} & = 0 \\
J_{53} & = 0 \\
J_{54} & = 0 \\
J_{55} & = -D \\
\end{align}


Evaluating the equilibrium point in the jacobian gives:

\textbf{Case 1}
\begin{align}
J = \begin{bmatrix}
0 & 0 &\dfrac{D(\bar{\mu}_1 - D)(s_{in}-\frac{K_1D}{\bar{\mu_1}-D})}{\bar{\mu}_1k_1} &0 &0 \\
0 & 0 & 0&  \dfrac{D(\bar{\mu}_2 - D)(s_{in}-\frac{K_1D}{\bar{\mu_1}-D} -\frac{K_2D}{\bar{\mu_2}-D})}{\bar{\mu}_2k_2} & 0 \\
-k_1D & 0& -D-\dfrac{D(\bar{\mu}_1 - D)(s_{in}-\frac{K_1D}{\bar{\mu_1}-D})}{\bar{\mu}_1} &0 &0 \\
k_1D & -k_2D & \dfrac{D(\bar{\mu}_1 - D)(s_{in}-\frac{K_1D}{\bar{\mu_1}-D})}{\bar{\mu}_1} & -D -\dfrac{D(\bar{\mu}_2 - D)(s_{in}-\frac{K_1D}{\bar{\mu_1}-D} -\frac{K_2D}{\bar{\mu_2}-D})}{\bar{\mu}_2} &0 \\
0 & 0 & 0 & 0 & -D 
\end{bmatrix}
\end{align}

\textbf{Case 2}


\end{document}          
